@prefix owl: <http://www.w3.org/2002/07/owl#> .
@prefix xsd: <http://www.w3.org/2001/XMLSchema#> .
@prefix dc: <http://purl.org/dc/terms/> .
@prefix rdfs: <http://www.w3.org/2000/01/rdf-schema#> .
@prefix rdf: <http://www.w3.org/1999/02/22-rdf-syntax-ns#> .
@prefix eeboo: <http://eeboo.oerc.ox.ac.uk/eeboo/> .
@prefix bf: <http://bibframe.org/vocab/> .
@prefix mads: <http://www.loc.gov/mads/rdf/v1#> .
@prefix mods: <http://www.loc.gov/mods/v3#> .

<http://eeboo.oerc.ox.ac.uk/eeboo>
  a owl:Ontology .
  
# Classes 
  
eeboo:Author
    a rdfs:Class ;
    rdfs:label "Author" ;
    rdfs:comment "A person who has created some form of work mentioned in the data and was mentioned in the work as the author" .

eeboo:Work
    a rdfs:Class ;
    rdfs:label "Work" ;
	owl:equivalentProperty bf:Instance ;
    rdfs:comment "A physical thing, the metadata details of which are captured in an object record such as an EEBO xml-file" .

eeboo:Entity_Printed_By
	a rdfs:Class ;
	rdfs:label "Entity_Printed_By" ;
	rdfs:comment "A named entity (person or organization) referred in the original data pulled from TEI as someone responsible for printing of the work" .

eeboo:Entity_Printed_For
	a rdfs:Class ;
	rdfs:label "Entity_Printed_For" ;
	rdfs:comment "A named entity (person or organization) referred in the original data pulled from TEI as someone who was probably responsible for subcommissioning the work, which can be for outsourcing, or supporting a (perhaps young, recently set up) fellow printer, or knowledge that a particular printer is skilled in setting a certain sort of text, or has a particular font, or that it was a joint endeavour. The relationship of this entity to the work is denoted as 'Printed for' in the data" .

eeboo:Entity_Sold_By
	a rdfs:Class ;
	rdfs:label "Entity_Sold_By" ;
	rdfs:comment "A named entity (person or organization) referred in the original data pulled from TEI as someone who was responsible for selling the work" .


#Properties
eeboo:raw_pubplace
  a rdf:Property, owl:DatatypeProperty ;
  rdfs:domain eeboo:Work ;
  rdfs:range xsd:string .

eeboo:precise-birth
  a rdf:Property, owl:DatatypeProperty ;
  rdfs:comment "The birth date of a person when it has been recorded without ambiguity or uncertainty" ;
  rdfs:domain eeboo:Author ;
  rdfs:label  "precise-date-of-birth"^^xsd:string;
  rdfs:range xsd:date .

eeboo:precise-death
    a rdf:Property, owl:DatatypeProperty ;
    rdfs:comment "The date of death of a person when it has been recorded without ambiguity or uncertainty" ;
    rdfs:domain eeboo:Author ;
    rdfs:label  "precise-date-of-death"^^xsd:string;
    rdfs:range xsd:date .
	
eeboo:approximate-birth
    a rdf:Property, owl:DatatypeProperty ;
    rdfs:comment "The birth date of a person when it has been recorded ambiguously or with a degree of uncertainty" ;
    rdfs:domain eeboo:Author ;
    rdfs:label  "approximate-date-of-birth"^^xsd:string;
    rdfs:range xsd:date .
  
eeboo:approximate-death
      a rdf:Property, owl:DatatypeProperty ;
      rdfs:comment "The date of death of a person when it has been recorded ambiguously or with a degree of uncertainty" ;
      rdfs:domain eeboo:Author ;
      rdfs:label  "approximate-date-of-death"^^xsd:string;
      rdfs:range xsd:date .
	  
eeboo:precise-floruit-start
      a rdf:Property, owl:DatatypeProperty ;
      rdfs:comment "The start date of a period of professional activity for a person when that time range has been recorded without ambiguity or uncertainty" ;
      rdfs:domain eeboo:Author ;
      rdfs:label  "precise-floruit-start"^^xsd:string;
      rdfs:range xsd:date .
	  
eeboo:precise-floruit-end
      a rdf:Property, owl:DatatypeProperty ;
      rdfs:comment "The end date of a period of professional activity for a person when that time range has been recorded without ambiguity or uncertainty" ;
      rdfs:domain eeboo:Author ;
      rdfs:label  "precise-floruit-end"^^xsd:string;
      rdfs:range xsd:date .
	  
eeboo:precise-publication
    a rdf:Property, owl:DatatypeProperty ;
    rdfs:comment "The publication date of a work when it has been recorded without ambiguity or uncertainty" ;
    rdfs:domain eeboo:Work ;
    rdfs:label  "precise-publication"^^xsd:string;
    rdfs:range xsd:date .
  
eeboo:approx-publication
    a rdf:Property, owl:DatatypeProperty ;
    rdfs:comment "The approximate publication date of a work i.e. when it has been recorded with ambiguity or uncertainty" ;
    rdfs:domain eeboo:Work ;
    rdfs:label  "precise-publication"^^xsd:string;
    rdfs:range xsd:date .

eeboo:creator
    a rdf:Property ;
    rdfs:domain eeboo:Work ;
    rdfs:label  "has_creator" ;
    owl:equivalentProperty dc:creator ;
    rdfs:range eeboo:Author .
	
eeboo:electronicLocation
	a rdf:Property ;
	rdfs:domain eeboo:Work ;
	rdfs:label  "electronic_representation_of_resource" ;
	rdfs:range xsd:string .

eeboo:hasExternalAuthorityVIAF
	a rdf:Property ;
	rdfs:domain eeboo:Author ;
	rdf:subPropertyOf mads:hasExactExternalAuthority ;
	rdfs:label  "Records the uri of the exact match entitity from VIAF" ;
	rdfs:range xsd:string .

eeboo:hasExternalAuthorityLoC
	a rdf:Property ;
	rdfs:domain eeboo:Author ;
	rdf:subPropertyOf mads:hasExactExternalAuthority ;
	rdfs:label  "Records the uri of the exact match entitity from Library of Congress" ;
	rdfs:range xsd:string .
	
eeboo:printedBy
	a rdf:Property ;
	rdfs:domain eeboo:Work ;
	rdfs:label "printed_by" ;
	rdfs:range eeboo:Entity_Printed_By .
	
eeboo:printedFor
	a rdf:Property ;
	rdfs:domain eeboo:Work ;
	rdfs:label "printed_for" ;
	rdfs:range eeboo:Entity_Printed_For .
	
	
eeboo:soldBy
	a rdf:Property ;
	rdfs:domain eeboo:Work ;
	rdfs:label "sold_by" ;
	rdfs:range eeboo:Entity_Sold_By .	
	


